some work on trying to get termination for Yul interpreter

YulSemantics.thy
@@ -29,14 +29,6 @@ definition restrict :: "'v local \<Rightarrow> 'v local \<Rightarrow> 'v local" 
   (if e2 i = None then None
       else e1 i)"
 
-(*
-fun il_length :: "identifier_list \<Rightarrow> nat" where
-"il_length (Ids _ l) = List.length l + 1"
-
-fun til_length :: "typed_identifier_list \<Rightarrow> nat" where
-"til_length (TIds _ l) = List.length l + 1"
-*)
-
 fun strip_id_type :: "YulTypedName \<Rightarrow> YulIdentifier" where
 "strip_id_type (YulTypedName name type) = name"
 
@@ -64,12 +56,6 @@ fun get_min :: "('a \<Rightarrow> nat) \<Rightarrow> 'a set \<Rightarrow> 'a" wh
 "get_min f aset =
   (SOME a . a \<in> aset \<and>
             (\<forall> a' \<in> aset . f a' \<le> f a \<longrightarrow> a = a'))"
-
-(* bogus temporary definition for "truthy" Yul values *)
-fun isTruthy :: "YulLiteralValue \<Rightarrow> bool" where
-"isTruthy str = 
-  (if str = STR ''0'' then False
-   else True)"
 
 datatype YulSwitchCanonical =
   YulSwitchCanonical
@@ -101,6 +87,9 @@ fun canonicalizeSwitch ::
     | Some (YulSwitchCanonical e cs' d') \<Rightarrow>
            Some (YulSwitchCanonical e ((YulSwitchCase (Some x) body)#cs') d'))"
 
+syntax plus_literal_inst.plus_literal :: "String.literal \<Rightarrow> String.literal \<Rightarrow> String.literal"
+  ("_ @@ _")
+
 (* executable semantics for Yul programs *)
 (* parameters:
    - global state
@@ -111,71 +100,165 @@ fun canonicalizeSwitch ::
 
 (* TODO: do we need to maintain the typing environment at runtime?
    I don't think we should. *)
-function yul_eval_statement :: 
-  "'g \<Rightarrow> YulLiteralValue local \<Rightarrow> function_sig local \<Rightarrow> YulStatement \<Rightarrow>
-   ('g * YulLiteralValue local * function_sig local * mode)"
+
+(* locale for fixing global state, value types *)
+locale YulSem =
+  fixes local_var :: "'v itself"
+  fixes local_type :: "'t itself"
+  fixes global_state :: "'g itself"
+
+  fixes gasCost :: "YulStatement \<Rightarrow> nat"
+  fixes gas :: "'g \<Rightarrow> nat"
+  fixes updateGas :: "nat \<Rightarrow> 'g \<Rightarrow> 'g"
+
+  fixes truthy :: "'v \<Rightarrow> bool"
+  (* for declared, undefined variables *)
+  fixes defaultValue :: "'v"
+  (* comparison of values for use in switch *)
+  fixes valueEq :: "'v \<Rightarrow> 'v \<Rightarrow> bool"
+
+  fixes error :: "String.literal \<Rightarrow> 'g \<Rightarrow> 'g"
+  fixes getError :: "'g \<Rightarrow> String.literal option"
+
+  (* TODO: probably need more primitives for type reasoning *)
+  fixes parseType :: "String.literal \<Rightarrow> 't option"
+  fixes parseLiteral :: "String.literal \<Rightarrow> 'v option"
+
+  assumes gas_decrease :
+    "\<And> s . gasCost s > 0"
+  assumes gas_lens1 :
+    "\<And> g . updateGas (gas g) g = g"
+  assumes gas_lens2 :
+    "\<And> n g . gas (updateGas n g) = n"
+  assumes gas_lens3 :
+    "\<And> n n' g . 
+      updateGas n (updateGas n' g) = updateGas n g"
+
+  assumes error_isError :
+    "\<And> msg G . getError (error msg G) = Some msg"    
+
+begin
+
+fun isError :: "'g \<Rightarrow> bool" where
+"isError G =
+  (case getError G of
+    None \<Rightarrow> False
+    | Some _ \<Rightarrow> True)"
+
+fun decrement_gas ::
+    "'g \<Rightarrow> YulStatement \<Rightarrow> 'g" where
+"decrement_gas G st =
+  (if gas G < gasCost st then error (STR ''Out of gas'') G
+   else updateGas (gas G - gasCost st) G)"
+
+lemma decrement_gas_correct :
+  assumes Ok : "\<not> isError G"
+  shows "isError (decrement_gas G st) \<or> gas (decrement_gas G st) < gas G"
+proof(cases "gas G < gasCost st")
+  case True
+
+  hence Bad : "isError (decrement_gas G st)"
+    by(simp add: error_isError)
+
+  thus ?thesis by auto
+next
+  case False
+
+  hence Good : "gas (decrement_gas G st) < gas G" using gas_decrease[of st]
+    by(simp add: gas_lens2)
+
+  thus ?thesis by auto
+qed
+
+
+(* gas checks will happen on statement *)
+function
+yul_eval_statement_check_gas ::
+    "'g \<Rightarrow> 'v local \<Rightarrow> function_sig local \<Rightarrow> YulStatement \<Rightarrow>
+    ('g * 'v local * function_sig local * mode)"
+and yul_eval_statement ::
+  "'g \<Rightarrow> 'v local \<Rightarrow> function_sig local \<Rightarrow> YulStatement \<Rightarrow>
+   ('g * 'v local * function_sig local * mode)"
 and yul_eval_statements ::
-  "'g \<Rightarrow> YulLiteralValue local \<Rightarrow> function_sig local \<Rightarrow> YulStatement list \<Rightarrow>
-   ('g * YulLiteralValue local * function_sig local * mode)"
+  "'g \<Rightarrow> 'v local \<Rightarrow> function_sig local \<Rightarrow> YulStatement list \<Rightarrow>
+   ('g * 'v local * function_sig local * mode)"
 and yul_eval_expression ::
-   "'g \<Rightarrow> YulLiteralValue local \<Rightarrow> function_sig local \<Rightarrow> YulExpression \<Rightarrow>
-   ('g * YulLiteralValue local * function_sig local * YulLiteralValue list)"
+   "'g \<Rightarrow> 'v local \<Rightarrow> function_sig local \<Rightarrow> YulExpression \<Rightarrow>
+   ('g * 'v local * function_sig local * 'v list)"
 and yul_eval_canonical_switch ::
- "'g \<Rightarrow> YulLiteralValue local \<Rightarrow> function_sig local \<Rightarrow> YulLiteralValue \<Rightarrow> YulSwitchCanonical \<Rightarrow>
-   ('g * YulLiteralValue local * function_sig local * mode)"  
+ "'g \<Rightarrow> 'v local \<Rightarrow> function_sig local \<Rightarrow> 'v \<Rightarrow> YulSwitchCanonical \<Rightarrow>
+   ('g * 'v local * function_sig local * mode)"  
 and yul_eval_args ::
-  "'g \<Rightarrow> YulLiteralValue local \<Rightarrow>
+  "'g \<Rightarrow> 'v local \<Rightarrow>
     function_sig local \<Rightarrow>
     YulExpression list \<Rightarrow>
-    ('g * YulLiteralValue local * function_sig local * YulLiteralValue list)" 
-where
+    ('g * 'v local * function_sig local * 'v list)" 
+  where
+
+(* gas checking (entry point) *)
+"yul_eval_statement_check_gas G L F st =
+  (let G' = decrement_gas G st in
+    (if isError G' then (G', L, F, Regular)
+     else yul_eval_statement G' L F st))"
 
 (*
  * helper: expression
  *)
 (* identifier *)
-"yul_eval_expression G L F (YulIdentifier i) =
+| "yul_eval_expression G L F (YulIdentifier i) =
  (case (L i) of
-  None \<Rightarrow> (G, L, F, undefined) \<comment> \<open>bogus error case \<close>
+  None \<Rightarrow> (error (STR ''Undefined variable '' @@ i) G, L, F, []) 
   | Some v \<Rightarrow> (G, L, F, [v]))"
 (* literal *)
 | "yul_eval_expression G L F (YulLiteralExpression (YulLiteral value type)) =
-   (G, L, F, [value])"
+  (case parseLiteral value of
+    Some v \<Rightarrow> (G, L, F, [v])
+    | None \<Rightarrow> (error (STR ''Bad literal '' @@ value) G, L, F, []))"
+
 (* function call *)
 (* TODO: evaluate function body as a block or as "raw" statements? *)
 | "yul_eval_expression G L F (YulFunctionCallExpression (YulFunctionCall name args)) =
    (case yul_eval_args G L F args of
     (G1, L1, F1, vals) \<Rightarrow>
       (case F1 name of
-        None \<Rightarrow> (G1, L1, F1, undefined) \<comment> \<open>bogus error case \<close>
+        None \<Rightarrow> (error (STR ''Undefined function '' @@ name) G1, L1, F1, [])
         | (Some (YulFunctionSig argSig retSig body)) \<Rightarrow>
           (case put_values local_empty (strip_id_types argSig) vals of
-          None \<Rightarrow> (G1, L1, F1, undefined) \<comment> \<open>bogus error case \<close>
+          None \<Rightarrow> (error (STR ''Argument arity mismatch for '' @@ name) G1, L1, F1, [])
           | Some Lsub \<Rightarrow>
-            (case put_values Lsub (strip_id_types retSig) (List.replicate (length retSig) 0) of
-            None \<Rightarrow> (G1, L1, F1, undefined) \<comment> \<open>bogus error case \<close>
-            | Some Lsub1 \<Rightarrow>
-              (case yul_eval_statement G1 Lsub1 F1 (YulBlock body) of
-                (G2, Lsub2, _, mode) \<Rightarrow>
-                (case get_values Lsub2 (strip_id_types retSig) of
-                  None \<Rightarrow> (G1, L1, F1, undefined) \<comment> \<open>bogus error case \<close>
-                  | Some retVals \<Rightarrow> (G2, L1, F1, retVals)))))))"
+            (case put_values Lsub (strip_id_types retSig) 
+                                  (List.replicate (length retSig) defaultValue) of
+              None \<Rightarrow> (error (STR ''Should be dead code'') G1, L1, F1, [])
+              | Some Lsub1 \<Rightarrow>
+                (case yul_eval_statement_check_gas G1 Lsub1 F1 (YulBlock body) of
+                  (G2, Lsub2, _, mode) \<Rightarrow> 
+                  (if isError G2 then (G2, L1, F1, [])
+                    else 
+                    (case get_values Lsub2 (strip_id_types retSig) of
+                      None \<Rightarrow> (error(STR ''Return arity mismatch for '' @@ name) G2, L1, F1, [])
+                      | Some retVals \<Rightarrow> (G2, L1, F1, retVals))))))))"
 
 (*
  * helper: "canonicalized" switch
+ *)
+(*
+ * TODO: handle gas consumption of switch cases
  *)
 | "yul_eval_canonical_switch G L F condValue
     (YulSwitchCanonical e [] dfl) =
     (yul_eval_statements G L F dfl)"
 (* canonicalization guarantees no defaults remain in cases list *)
 | "yul_eval_canonical_switch G L F condValue
-    (YulSwitchCanonical e (YulSwitchCase None _ # _) _) = undefined"
+    (YulSwitchCanonical e (YulSwitchCase None _ # _) _) = 
+    (error (STR ''Non canonical switch statement'') G, L, F, Regular)"
 | "yul_eval_canonical_switch G L F condValue
     (YulSwitchCanonical e (YulSwitchCase (Some (YulLiteral hdValue _)) hdBody # rest) dfl) =
-    (if hdValue = condValue
-     then yul_eval_statements G L F hdBody
-     else yul_eval_canonical_switch G L F condValue (YulSwitchCanonical e rest dfl))
-    "
+    (case parseLiteral hdValue of
+      None \<Rightarrow> (error (STR ''Bad literal '' @@ hdValue) G, L, F, Regular)
+      | Some v \<Rightarrow>
+        (if valueEq v condValue
+         then yul_eval_statements G L F hdBody
+         else yul_eval_canonical_switch G L F condValue (YulSwitchCanonical e rest dfl)))"
 
 (* 
  * helper: statement list
@@ -183,7 +266,9 @@ where
 | "yul_eval_statements G L F [] = (G, L, F, Regular)"
 | "yul_eval_statements G L F (sh#st) =
    (case yul_eval_statement G L F sh of
-    (G1, L1, F1, Regular) \<Rightarrow> yul_eval_statements G1 L1 F1 st
+    (G1, L1, F1, Regular) \<Rightarrow> 
+      (if isError G1 then (G1, L1, F1, Regular)
+       else yul_eval_statements G1 L1 F1 st)
     | (G1, L1, F1, mode) \<Rightarrow> (G1, L1, F1, mode))"
 
 (*
@@ -195,7 +280,7 @@ where
       (G1, L1, F1, [vh]) \<Rightarrow>
         (case yul_eval_args G1 L1 F1 et of
           (Gn, Ln, Fn, vt) \<Rightarrow> (Gn, Ln, Fn, vh#vt))
-      | _ \<Rightarrow> undefined)"
+      | _ \<Rightarrow> (error (STR ''Expression doesn't have 1 value (function argument)'') G, L, F, []))"
 
 (*
  * statement
@@ -225,10 +310,12 @@ to propagate back up to outer scopes? this seems bad *)
    if we have Some, then evaluate it as an assignment *)
 | "yul_eval_statement G L F
     (YulVariableDeclarationStatement (YulVariableDeclaration names None)) =
-  (case put_values L (strip_id_types names) (List.replicate (length names) undefined) of
-    None \<Rightarrow> (G, L, F, Regular) \<comment> \<open>bogus error case \<close>
+  (case put_values L (strip_id_types names) (List.replicate (length names) defaultValue) of
+    None \<Rightarrow> (error (STR ''Should be dead code'') G, L, F, Regular)
     | Some L1 \<Rightarrow>  (G, L1 , F, Regular))"
+
 (* variable declaration + definition *)
+(* TODO: do we need to check gas again? i don't think we should. *)
 | "yul_eval_statement G L F
     (YulVariableDeclarationStatement (YulVariableDeclaration names (Some expr))) =
    yul_eval_statement G L F (YulAssignmentStatement (YulAssignment (strip_id_types names) expr))"
@@ -246,9 +333,9 @@ to propagate back up to outer scopes? this seems bad *)
 | "yul_eval_statement G L F (YulIf cond body) =
    (case yul_eval_expression G L F cond of
     (G1, L1, F1, [v]) \<Rightarrow>
-      (if isTruthy v then yul_eval_statements G L F body
+      (if truthy v then yul_eval_statements G L F body
        else (G, L, F, Regular))
-    | _ \<Rightarrow> undefined)"
+    | _ \<Rightarrow> (error (STR ''Expression doesn't have 1 value (if condition)'') G, L, F, Regular))"
 
 (* for loops *)
 
@@ -256,7 +343,7 @@ to propagate back up to outer scopes? this seems bad *)
 | "yul_eval_statement G L F (YulForLoop [] cond post body) =
    (case yul_eval_expression G L F cond of
     (G1, L1, F1, [v]) \<Rightarrow>
-      (if isTruthy v
+      (if truthy v
        then
         (case yul_eval_statements G1 L F1 body of
          (G2, L2, F2, mode) \<Rightarrow>
@@ -267,11 +354,13 @@ to propagate back up to outer scopes? this seems bad *)
                   (G3, L3, F3, mode) \<Rightarrow>
                   (case mode of
                     Leave \<Rightarrow> (G2, L3, F2, Leave)
-                    | _ \<Rightarrow> yul_eval_statement G3 L3 F3 (YulForLoop [] cond post body)))))
+                    | _ \<Rightarrow> yul_eval_statement_check_gas G3 L3 F3 (YulForLoop [] cond post body)))))
        else (G1, L1, F1, Regular))
       | _ \<Rightarrow> undefined)"
      
 (* process pre-statements for for-loop *)
+(* TODO: I don't think we need to deduct gas when we do the final yul_eval_statement call
+   because all we have done here is preprocess the loop structure *)
 | "yul_eval_statement G L F (YulForLoop (preh#pret) cond post body) =
    (case yul_eval_statements G L F (preh#pret) of
         (G1, L1, F1, mode) \<Rightarrow>
@@ -302,11 +391,6 @@ to propagate back up to outer scopes? this seems bad *)
 (* leave *)
 | "yul_eval_statement G L F YulLeave = (G, L, F, Leave)"
 
-(* locale for fixing global state, value types *)
-locale YulSem =
-  fixes v_int :: "int \<Rightarrow> 'v"
-  fixes v_get_int :: "'v \<Rightarrow> int option"
-begin
 
 (* big-step inductive semantics for Yul programs *)
 (* parameters:
@@ -318,6 +402,28 @@ begin
 (* NB official Yul interpreter appears to be
 registering functions at the block level, rather than
 as they appear syntactically.
+*)
+  by pat_completeness auto
+
+
+(* measure for yul_eval function - based on gas *)
+(* however we are also going to need a notion of how far in the syntax tree we are.
+   then we should only need to use gas for the for loop piece *)
+
+(*
+termination
+  apply(relation 
+      "measure 
+        (\<lambda> x .
+          (case x of
+              Inl (Inl (G, L, F, st)) \<Rightarrow> 0
+              | Inl (Inr (Inl (G, L, F, st))) \<Rightarrow> 0
+              | Inl (Inr (Inr (G, L, F, sts))) \<Rightarrow> 0
+              | Inr (Inl (G, L, F, e)) \<Rightarrow> 0
+              | Inr (Inr (Inl (G, L, F, sw))) \<Rightarrow> 0
+              | Inr (Inr (Inr (G, L, F, args))) \<Rightarrow> 0))")
+  apply(simp_all)
+end
 *)
 
 end
